examples/ring/RingIAproof.v
@@ -1,0 +1,468 @@
+Require Import Coqlib ITreelib sflib.
+Require Import SMod ModSim.
+Require Import ImpPrelude.
+Require Import Skeleton.
+Require Import PCM IPM IFacts.
+Require Import Events Behavior.
+Require Import Relation_Definitions.
+
+(*** TODO: export these in Coqlib or Universe ***)
+Require Import Relation_Operators.
+Require Import RelationPairs.
+From ITree Require Import
+     Events.MapDefault.
+From ExtLib Require Import
+     Core.RelDec
+     Structures.Maps
+     Data.Map.FMapAList.
+Require Import Mem1 STB.
+
+Require Import ISim HMod Events.
+Require Import Mod ModSimFacts.
+Require Import CellHeader CellASpec CellA RingHeader RingA RingASpec CtrlI.
+
+Set Implicit Arguments.
+
+Local Open Scope nat_scope.
+
+Section XXX.
+  Context `{Σ: GRA.t}.
+Definition HModSem_empty: HModSem.t :=
+  {| HModSem.fnsems := [];
+     HModSem.initial_st := tt↑;
+     HModSem.initial_cond := emp |}.
+Definition HMod_empty: HMod.t :=
+  {|HMod.get_modsem := fun _ => HModSem_empty; HMod.sk := [] |}.
+
+(* Fixpoint hmod_addL (l: list HMod.t) : HMod.t := *)
+(*   match l with *)
+(*   | [] => HMod_empty *)
+(*   | m :: l' => HMod.add m (hmod_addL l') *)
+(*   end. *)
+
+End XXX.
+
+
+  
+
+Module RingIA.
+Section SIMMODSEM.
+  Context `{Σ: GRA.t}.
+  Context `{_M: CellRA.t (Σ:=Σ)}.
+  
+  Variable max_size : nat.
+
+  Variable StbA: Sk.t -> gname -> option fspec.
+  Hypothesis RingInStb: forall sk, stb_incl (to_stb RingAS.Stb) (StbA sk).
+  Hypothesis CellInStb: forall sk idx (LT: idx < max_size), stb_incl (to_stb (CellAS.Stb idx)) (StbA sk).
+
+  Import CellAS.
+
+  Local Notation RingAMod := (RingA.t max_size StbA).
+  Local Notation CtrlIMod := (CtrlI.t max_size).
+  Local Notation CellAMod := (fun i => CellA.t i StbA).
+
+  Fixpoint CellGroup max :=
+    match max with
+    | 0 => HMod_empty
+    | S max' => HMod.add (CellAMod max' ) (CellGroup max')
+    end.
+  
+  Local Notation RingIMod := (HMod.add CtrlIMod (CellGroup max_size)).
+
+  Definition rotate_rev {T} n (l: list T) :=
+    drop ((strings.length l)-(n mod strings.length l)) l ++ take ((strings.length l)-(n mod strings.length l)) l.
+
+  Lemma rotate_rev_inv {T} n (l: list T):
+    rotate_rev n (rotate n l) = l.
+  Proof. admit. Admitted.
+
+  Lemma rotate_rev_id {T} (l: list T):
+    rotate_rev 0 l = l.
+  Proof. admit. Admitted.
+  
+  Definition Ist: Any.t -> Any.t -> iProp :=
+    (fun st_src st_tgt =>
+       ((∃ (sz:nat) (q q': list Z) (hd tl: nat) cell_state,
+         ⌜st_src = (sz, q)↑ /\ List.length q = sz /\ sz < max_size /\
+          st_tgt = Any.pair (hd,tl)↑ cell_state /\ hd-tl = sz /\
+          List.length (q ++ q') = max_size⌝ ∗
+          [∗ list] i↦x ∈ rotate_rev tl (q++q'), (CellAS.pending i ∨ CellAS.cell (i mod max_size) x))))%I.
+
+  Variable fl: alist string (Any.t → itree hmodE Any.t).
+  Variable fr: alist string (Any.t → itree hmodE Any.t).
+
+Ltac init_simF := let name := fresh "name" in
+  unfold HModR.sim_fun; i;
+  do 2 match goal with
+  | [|-context[alist_find _ (_ (_ (HMod.add ?x _) _))]] => rewrite/__ {1}/x
+  | [|-context[alist_find _ (_ (_ ?x _))]] => rewrite/__ {1}/x
+  end;
+  unseal "ccr";
+  alist_find_solver;
+  repeat match goal with
+  | [|- context[{| fsb_body := cfunU ?x |}]] => rewrite/__ {1}/x
+  | [|- context[cfunU ?x]] => rewrite/__ {1}/x
+  end;
+  unfold interp_sb_hp, HoareFun, cfunU, ccallU; s;
+  ii; subst; iIntros "IST".
+
+Ltac hss :=
+  ss;
+  try (unfold run_l, run_r in *; rewrite !Any.pair_split in *; fold run_l run_r in * );
+  try (rewrite !Any.upcast_downcast in * );
+  (repeat match goal with [G: Any.downcast _ = Some _ |-_] =>
+    apply Any.downcast_upcast in G; inv G; ss
+   end);
+  (repeat match goal with [G: Any.upcast (_:?T) = Any.upcast (_:?T) |-_] =>
+    apply Any.upcast_inj in G; destruct G as [_ G]; red in G; depdes G; ss
+   end);
+  (repeat match goal with [G: Some _ = Some _ |- _] =>
+    depdes G; ss
+   end).
+
+Ltac inv_string X :=
+  inv X;
+  repeat match goal with [H: @eq string (_ ++ _)%string (_ ++ _)%string|-_] =>
+           apply string_app_inv in H
+    end; ss.
+
+Ltac alist_find_solver :=
+  match goal with [|-context[alist_find ?x]] => rewrite <-(Seal.sealing_eq "_tmp_" x) end;
+  s; unfold rel_dec, Dec_RelDec, sumbool_to_bool, dec, string_Dec;
+  des_ifs; unseal "_tmp_";
+  repeat match goal with [H: @eq string _ _|-_] => inv_string H end;
+  repeat match goal with [H: not (@eq string _ _)|-_] => clear H end.
+
+
+
+
+
+Lemma string_app_length s1 s2:
+  length (s1++s2)%string = length s1 + length s2.
+Proof.
+  induction s1.
+  - unfold append; fold append. eauto.
+  - s. fold append. rewrite IHs1. nia.
+Qed.
+
+Lemma string_app_inv_r
+  p s s'
+  (EQ: (s ++ p = s' ++ p)%string)
+  :
+  (s = s')%string.
+Proof.
+  revert p s' EQ. induction s; i; ss.
+  { destruct s'; eauto.
+    apply (f_equal length) in EQ.
+    rewrite !string_app_length in EQ. ss. nia. }
+  destruct s'.
+  { apply (f_equal length) in EQ.
+    rewrite !string_app_length in EQ. ss. nia. }
+  revert EQ. unfold append; fold append. i.
+  inv EQ. f_equal. eauto.
+Qed.
+
+Lemma list_ascii_of_string_app s1 s2:
+  list_ascii_of_string (s1 ++ s2)%string =
+    list_ascii_of_string s1 ++ list_ascii_of_string s2.
+Proof.
+  revert s2. induction s1; i; s; eauto.
+  rewrite IHs1; eauto.
+Qed.
+
+Lemma string_of_list_ascii_app l1 l2:
+  string_of_list_ascii (l1 ++ l2) =
+    (string_of_list_ascii l1 ++ string_of_list_ascii l2)%string.
+Proof.
+  revert l2. induction l1; i; s; eauto.
+  rewrite IHl1. eauto.
+Qed.
+
+(* Lemma string_app_nil s: *)
+(*   (s ++ "")%string = s. *)
+(* Proof. *)
+(*   induction s; eauto. *)
+(*   unfold append; fold append. rewrite IHs; eauto. *)
+(* Qed. *)
+
+(* Lemma string_rev_app_inv_r *)
+(*   (s1 s2 s3: string) *)
+(*   (EQ: string_rev_app s1 s3 = string_rev_app s2 s3) *)
+(*   : *)
+(*   s1 = s2. *)
+(* Proof. *)
+(*   revert s2 s3 EQ. induction s1; i; ss. *)
+(*   - Check string_rev_app. *)
+
+(* Qed. *)
+
+(* string_of_list_ascii_of_string: *)
+(*   ∀ s : string, string_of_list_ascii (list_ascii_of_string s) = s *)
+(* list_ascii_of_string_of_list_ascii: *)
+(*   ∀ s : list Ascii.ascii, list_ascii_of_string (string_of_list_ascii s) = s *)
+
+(* Lemma string_app_rev *)
+(*   (s s': string) *)
+(*   : *)
+(*   (string_rev (s ++ s') = string_rev s' ++ string_rev s)%string. *)
+(* Proof. *)
+(*   revert s'; induction s; s; i. *)
+(*   { unfold append; fold append. *)
+(*     unfold string_rev; s. *)
+(*     Search (_++_)%string. *)
+(* Qed. *)
+
+(* Definition name_prefix (i: nat) (name: string) := *)
+(*   HexString.of_nat i +:+ ":" +:+ name. *)
+
+  Lemma string_of_nat_prefix_eq idx1 idx2 method1 method2
+    (EQ: (HexString.of_nat idx1 ++ "." ++ method1 =
+          HexString.of_nat idx2 ++ "." ++ method2)%string)
+    :
+    idx1 = idx2.
+  Proof.
+  Admitted.
+
+  Lemma cell_name_neq idx idx' method
+    (NEQ: idx ≠ idx') sk
+    :
+    alist_find (CellName.mk idx method) (List.map HModSem.trans_r
+      (HModSem.fnsems (HMod.get_modsem (CellA.t idx' StbA) sk))) = None.
+  Proof.
+    unfold CellA.t. unseal "ccr". s.
+    unfold rel_dec, Dec_RelDec, sumbool_to_bool, dec, string_Dec.
+    des_ifs; exfalso; apply string_of_nat_prefix_eq in H1; ss.
+  Qed.
+
+  Fixpoint emb_rec n fns :=
+    match n with
+    | 0 => List.map HModSem.trans_l fns
+    | S n' => List.map HModSem.trans_r (emb_rec n' fns)
+    end.
+  
+  (* Lemma cell_name_find max idx method *)
+  (*   (LT: idx < max) sk *)
+  (*   : *)
+  (*   alist_find (CellName.mk idx method) (List.map HModSem.trans_r *)
+  (*     (HModSem.fnsems (HMod.get_modsem (CellGroup max) sk))) *)
+  (*   = *)
+  (*   alist_find (CellName.mk idx method) (List.map HModSem.trans_r *)
+  (*     (HModSem.fnsems (HMod.get_modsem (CellA.t idx StbA) sk))). *)
+  (* Proof. *)
+  (*   revert_until max. clear -max. induction max; i. *)
+  (*   { nia. } *)
+  (*   assert (idx = max \/ idx < max) by nia. des; subst. *)
+  (*   { s. unfold HModSem.add_fnsems. rewrite List.map_app. *)
+  (*     destruct (alist_find (CellName.mk max method) *)
+  (*                 (List.map HModSem.trans_r *)
+  (*                    (HModSem.fnsems (HMod.get_modsem (CellA.t max StbA) sk)))) eqn: EQ. *)
+  (*     - eapply alist_find_app. rewrite List.map_map. *)
+        
+  (*       Search alist_find. *)
+
+
+
+  (*     unfold CellA.t. unseal "ccr". *)
+  (* match goal with [|-context[alist_find ?x]] => rewrite <-(Seal.sealing_eq "_tmp_" x) end. *)
+  (* s; unfold rel_dec, Dec_RelDec, sumbool_to_bool, dec, string_Dec; *)
+  (* des_ifs; unseal "_tmp_". *)
+  (* + exfalso. inv e. *)
+  (*   apply (f_equal list_ascii_of_string) in H1. *)
+  (*   rewrite !list_ascii_of_string_app in H1. *)
+  (*   apply (f_equal (@rev _)) in H1. *)
+  (*   rewrite !rev_app_distr in H1. *)
+  (*   apply app_inv_head in H1. *)
+  (*   apply (f_equal (@rev _)) in H1. *)
+  (*   rewrite !rev_involutive in H1. *)
+  (*   apply (f_equal string_of_list_ascii) in H1. *)
+  (*   rewrite !string_of_list_ascii_of_string in H1. *)
+  (*   apply (f_equal HexString.to_nat) in H1. *)
+  (*   rewrite !HexString.to_nat_of_nat in H1. nia. *)
+  (* + exfalso. inv e. *)
+  (*   apply (f_equal list_ascii_of_string) in H1. *)
+  (*   rewrite !list_ascii_of_string_app in H1. *)
+  (*   apply (f_equal (@rev _)) in H1. *)
+  (*   rewrite !rev_app_distr in H1. ss. *)
+  (* + *)
+    
+
+  (*   Search string. *)
+
+
+  (*   Require Import HexString. *)
+
+
+  (*   apply string_app_inv_r in H1. *)
+  (*   apply (f_equal HexString.to_nat) in H1. *)
+  (*   rewrite !HexString.to_nat_of_nat in H1. nia. *)
+
+    
+  
+  
+
+  (* apply string_app_inv in H1. *)
+  
+  (* try match goal with [H: @eq string _ _|-_] => inv_string H end. *)
+
+
+
+  
+  (* repeat match goal with [H: not (@eq string _ _)|-_] => clear H end *)
+    
+  (*   destruct idx. *)
+  (*   - *)
+
+    
+  (*   - destruct max_size eqn: EQ; try nia. s. rewrite EQ. *)
+  (*     unfold CellA.t. unseal "ccr". *)
+
+  (* match goal with [|-context[alist_find ?x]] => rewrite <-(Seal.sealing_eq "_tmp_" x) end. *)
+  (* s; unfold rel_dec, Dec_RelDec, sumbool_to_bool, dec, string_Dec. *)
+  (* des_ifs; unseal "_tmp_". *)
+
+  
+
+  
+  
+  (* repeat match goal with [H: @eq string _ _|-_] => inv_string H end. *)
+
+
+  
+  (* repeat match goal with [H: not (@eq string _ _)|-_] => clear H end. *)
+      
+  (*     alist_find_solver. *)
+      
+      
+    
+    
+  (* Qed. *)
+
+(*   Lemma simF_init: *)
+(*     HModR.sim_fun RingAMod RingIMod Ist RingName.init. *)
+(*   Proof. *)
+(*     init_simF. *)
+
+(*     st_l. iDestruct "ASM" as "%". subst. hss. *)
+(*     iDestruct "IST" as (sz q q' hd tl cell_state) "(% & CS)". des; subst. *)
+
+(*     st_r. force_l. st_l. force_l. *)
+(*     iSplitL "". { eauto. } *)
+
+(*     st. *)
+(*     iSplitL; eauto. *)
+(*     iExists 0, [], (rotate_rev tl (q++q')%list), 0, 0, cell_state. s. *)
+(*     replace (rotate_rev 0 (rotate_rev tl (q ++ q'))) with *)
+(*       (rotate_rev tl (q ++ q')) by admit. *)
+(*     iFrame. hss. *)
+(*     iPureIntro. esplits; eauto; try nia. *)
+(*     admit. *)
+(*   Admitted. *)
+
+(*   Lemma simF_dequeue: *)
+(*     HModR.sim_fun RingAMod RingIMod Ist RingName.dequeue. *)
+(*   Proof. *)
+(*     init_simF. *)
+
+(*     st_l. iDestruct "ASM" as "%". subst. hss. *)
+(*     iDestruct "IST" as (sz q q' hd tl cell_state) "(% & CS)". des; subst. *)
+(*     st_l. st_r. hss. rewrite <-H4. destruct (hd-tl) eqn: EQ; s. *)
+(*     { st. do 2 force_l. iSplitL ""; eauto. *)
+(*       st. iSplitL; eauto. unfold Ist. *)
+(*       iExists _,_,_,_,_,_. iFrame. *)
+(*       iPureIntro. esplits; eauto. nia. *)
+(*     } *)
+
+(*     st_r. *)
+(*     inline_r. *)
+(*     { unfold CtrlIMod. unseal "ccr". hide_evars. *)
+(*       alist_find_solver. show_evars. *)
+      
+      
+
+(*   match goal with [|-context[alist_find ?x]] => rewrite <-(Seal.sealing_eq "_tmp_" x) end. *)
+(*   s; unfold rel_dec, Dec_RelDec, sumbool_to_bool, dec, string_Dec. *)
+(*   des_ifs. unseal "_tmp_". *)
+(*   repeat match goal with [H: @eq string _ _|-_] => inv_string H end; *)
+(*   repeat match goal with [H: not (@eq string _ _)|-_] => clear H end       *)
+(*       alist_find_solver. *)
+
+      
+(*   Smatch goal with [|-context[alist_find ?x]] => rewrite <-(Seal.sealing_eq "_tmp_" x) end. *)
+(*   s; unfold rel_dec, Dec_RelDec, sumbool_to_bool, dec, string_Dec. *)
+(*   des_ifs; unseal "_tmp_". *)
+  
+(*   repeat match goal with [H: @eq string _ _|-_] => inv_string H end. *)
+(*   repeat match goal with [H: @eq string _ _|-_] => inv_string H end. *)
+(*   repeat match goal with [H: @eq string _ _|-_] => inv_string H end. *)
+(*   repeat match goal with [H: @eq string _ _|-_] => inv_string H end. *)
+
+  
+
+  
+(*   repeat match goal with [H: (_: string) ≠ _|-_] => clear H end. *)
+
+      
+
+
+    
+    
+(* exfalso. *)
+
+
+
+    
+    
+
+
+
+(*     force_l. st_l. force_l. *)
+(*     iSplitL "". { eauto. } *)
+    
+(*     st_l. iDestruct "ASM" as "((% & C) & %)". *)
+(*     subst. hss. rename y0 into v. unfold Ist. *)
+(*     iDestruct "IST" as "[(C0 & _)|(P & IST)]". *)
+(*     { iExFalso. iApply (cell_unique with "C0 C"). } *)
+(*     iDestruct "IST" as (v') "(A & %)". subst. hss. *)
+
+(*     iPoseProof (cell_auth_get with "C A") as "%". subst. *)
+
+(*     st_r. force_l. st_l. force_l. force_l. *)
+(*     iSplitL "C". { eauto. } *)
+
+(*     st. iSplitL; [|eauto]. *)
+(*     iRight. iFrame. eauto. *)
+(*   Qed. *)
+  
+(*   Lemma simF_set: *)
+(*     HModR.sim_fun CellAMod CellIMod Ist (CellName.set idx). *)
+(*   Proof. *)
+(*     init_simF. *)
+    
+(*     st_l. hss. iDestruct "ASM" as "((% & C) & %)". *)
+(*     subst. hss. rename y1 into v, y2 into v0. unfold Ist. *)
+(*     iDestruct "IST" as "[(C0 & _)|(P & IST)]". *)
+(*     { iExFalso. iApply (cell_unique with "C0 C"). } *)
+(*     iDestruct "IST" as (v') "(A & %)". subst. hss. *)
+
+(*     iPoseProof (cell_auth_get with "C A") as "%". subst. *)
+(*     iMod (cell_auth_set with "C A") as "(C & A)". *)
+    
+(*     st_r. force_l. st_l. force_l. force_l. *)
+(*     iSplitL "C". { eauto. } *)
+
+(*     st. iSplitL; [|eauto]. *)
+(*     iRight. iFrame. eauto. *)
+(*   Qed. *)
+
+(*   Theorem sim: HModR.sim CellAMod CellIMod Ist. *)
+(*   Proof. *)
+(*     init_sim. *)
+(*     - unfold Ist. eauto. *)
+(*     - use_simF simF_init. *)
+(*     - use_simF simF_get. *)
+(*     - use_simF simF_set. *)
+(*   Qed. *)
+
+End SIMMODSEM.
+End RingIA.
